a prototype version

otbn_model/code/modexp_var_lemmas.dfy
@@ -11,6 +11,65 @@ module modexp_var_lemmas {
     import opened mont_loop_lemmas
     import opened montmul_lemmas
 
+    predicate subb_inv(
+        dst: seq<uint256>,
+        carry: uint1,
+        src1: seq<uint256>,
+        src2: seq<uint256>,
+        index: nat)
+
+    requires |dst| == |src1| == |src2|;
+    requires index <= |src1|;
+    {
+        (dst[..index], carry)
+            == seq_subb(src1[..index], src2[..index])
+    }
+
+    lemma subb_inv_peri_lemma(
+        dst: seq<uint256>,
+        new_carry: uint1,
+        src1: seq<uint256>,
+        src2: seq<uint256>,
+        old_carry: uint1,
+        index: nat)
+    requires |dst| == |src1| == |src2|;
+    requires index < |src1|;
+    requires subb_inv(dst, old_carry, src1, src2, index);
+    requires (dst[index], new_carry)
+        == uint256_subb(src1[index], src2[index], old_carry);
+    ensures subb_inv(dst, new_carry, src1, src2, index + 1);
+    {
+        var (zs, bin) := seq_subb(src1[..index], src2[..index]);
+        var (z, bout) := uint256_subb(src1[index], src2[index], old_carry);
+
+        assert dst[..index+1] == zs + [z];
+        assert src1[..index+1] == src1[..index] + [src1[index]];
+        assert src2[..index+1] == src2[..index] + [src2[index]];
+    }
+
+    lemma subb_inv_post_lemma(
+        dst: seq<uint256>,
+        carry: uint1,
+        src1: seq<uint256>,
+        src2: seq<uint256>)
+        
+    requires |dst| == |src1| == |src2|;
+    requires subb_inv(dst, carry, src1, src2, |dst|);
+    ensures carry == 0 ==> to_nat(src1) - to_nat(src2) == to_nat(dst);
+    ensures carry == 1 ==> to_nat(src1) < to_nat(src2);
+    {
+        var index := |dst|;
+        assert dst[..index] == dst;
+        assert src1[..index] == src1;
+        assert src2[..index] == src2;
+    
+        seq_subb_nat_lemma(src1, src2, dst, carry);
+
+        assert to_nat(src1) - to_nat(src2) + carry * pow_B256(index) == to_nat(dst);
+
+        to_nat_bound_lemma(dst);
+    }
+
     predicate modexp_var_inv(
         a: nat,
         sig: nat,
@@ -27,9 +86,9 @@ module modexp_var_lemmas {
         sig: seq<uint256>,
         key: pub_key)
 
-        requires montmul_inv(a_slice, rr, NUM_WORDS, sig, key);
-        requires to_nat(rr) == key.RR;
-        ensures modexp_var_inv(to_nat(a_slice), to_nat(sig), 0, key);
+    requires montmul_inv(a_slice, rr, NUM_WORDS, sig, key);
+    requires to_nat(rr) == key.RR;
+    ensures modexp_var_inv(to_nat(a_slice), to_nat(sig), 0, key);
     {
         var m := key.m;
         var a := to_nat(a_slice);
@@ -142,6 +201,48 @@ module modexp_var_lemmas {
             cong(next_a, power(s, power(2, key.e') + 1), m);
             cong(next_a, power(s, key.e), m);
             cong(to_nat(next_a_slice), power(to_nat(sig), key.e), m);
+        }
+
+    }
+
+    function mod(a: int, n: nat): int
+        requires n != 0;
+    {
+        a % n
+    }
+
+    lemma modexp_var_correct_lemma(
+        raw_val: nat,
+        adjusted_val: nat,
+        carry: bool,
+        sig: nat,
+        key: pub_key)
+
+    requires pub_key_inv(key);
+    requires raw_val < sig + key.m;
+    requires cong(raw_val, power(sig, key.e), key.m);
+    requires carry ==> raw_val < key.m;
+    requires !carry ==> raw_val - key.m == adjusted_val;
+
+    ensures carry ==> raw_val == power(sig, key.e) % key.m;
+    ensures !carry ==> adjusted_val == power(sig, key.e) % key.m;
+    {
+        if carry {
+            cong_remainder_lemma(raw_val, power(sig, key.e), key.m);
+            assert raw_val == power(sig, key.e) % key.m;
+        } else {
+            assume sig < key.m; // TODO: fix this
+            calc ==> {
+                true;
+                    { cong_add_lemma_3(raw_val, -(key.m as int), key.m); }
+                cong(raw_val, adjusted_val, key.m);
+                    {
+                        cong_trans_lemma(adjusted_val, raw_val, power(sig, key.e), key.m);
+                    }
+                cong(adjusted_val, power(sig, key.e), key.m);
+            }
+
+            cong_remainder_lemma(adjusted_val, power(sig, key.e), key.m);
         }
     }
 }
